add start of eval_lvalue, add type_args to builtin funcs, flesh out intexample

deps/poulet4/examples/IntExample.v
@@ -16,8 +16,8 @@ Definition constTyp : P4Type := TypInteger.
 Definition name : P4String tag_t := MkP4String tag_t tag (caml_string_of_chars "hello_world").
 Definition value : ValueBase tag_t := ValBaseInteger tag_t 42.
 
-Definition parses (p: ValueObject tag_t) (fuel: nat) (start: caml_string): bool :=
-  match run_with_state nil (step_trans tag_t tag p fuel start) with
+Definition parses (p: ValueObject tag_t) (fuel: nat) (start_state: caml_string) (start_env: Environment.environment tag_t): bool :=
+  match run_with_state start_env (step_trans tag_t tag p fuel start_state) with
   | (inl _, _) => true
   | _ => false
   end.
@@ -36,19 +36,18 @@ parser IntExample (packet_in pkt, out int output) {
 }
 *)
 
-(* TODO: I'm pretty sure this scope needs to be legit and needs definitions for pkt and output, so something like
-  scope_pkt_3 := [pkt |-> Packet [1;1], output |-> 0]
-*)
 Definition scope : Env_EvalEnv := MkEnv_EvalEnv nil nil (caml_string_of_chars "dummy").
+(* Definition good_scope : Env_EvalEnv := MkEnv_EvalEnv  *)
 
 Definition pkt_param : P4Parameter := MkParameter true Directionless (TypExtern (caml_string_of_chars "packet_in")) (caml_string_of_chars "pkt").
-Definition out_param : P4Parameter := MkParameter true Out TypInteger (caml_string_of_chars "output").
+Definition out_type : P4Type := TypInt 2.
+Definition out_param : P4Parameter := MkParameter true Out out_type (caml_string_of_chars "output").
 Definition locals : list (Declaration tag_t) := nil.
 Definition accept_st : ParserState tag_t := MkParserState _ tt (MkP4String _ tt StrConstants.accept) nil (ParserDirect _ tt (MkP4String _ tt StrConstants.accept)).
-Definition output_expr : Expression tag_t := MkExpression _ tt (ExpName _ (BareName (caml_string_of_chars "output"))) TypInteger Directionless.
-Definition pkt_extract_expr : Expression tag_t := MkExpression _ tt (ExpName _ (BareName (caml_string_of_chars "pkt"))) (TypFunction (MkFunctionType nil ((MkParameter false Directionless TypInteger (caml_string_of_chars "x"))::nil) FunBuiltin TypInteger)) Directionless.
+Definition output_expr : Expression tag_t := MkExpression _ tt (ExpName _ (BareName (caml_string_of_chars "output"))) out_type Directionless.
+Definition pkt_extract_expr : Expression tag_t := MkExpression _ tt (ExpName _ (BareName (caml_string_of_chars "pkt"))) (TypFunction (MkFunctionType nil ((MkParameter false Directionless out_type (caml_string_of_chars "x"))::nil) FunBuiltin out_type)) Directionless.
 Definition extract_stmt : Statement tag_t := 
-  MkStatement _ tt (StatMethodCall _ (MkExpression _ tt (ExpExpressionMember _ pkt_extract_expr (MkP4String _ tt StrConstants.extract)) TypVoid Directionless) nil nil) StmVoid.
+  MkStatement _ tt (StatMethodCall _ (MkExpression _ tt (ExpExpressionMember _ pkt_extract_expr (MkP4String _ tt StrConstants.extract)) TypVoid Directionless) (out_type :: nil) (Some output_expr :: nil)) StmVoid.
 
 
 Definition body: list (Statement tag_t) := extract_stmt :: nil.
@@ -58,18 +57,210 @@ Definition states : list (ParserState tag_t) := start_st :: nil.
 
 Definition IntParser : ValueObject tag_t := ValObjParser _ scope nil nil states.
 
-Lemma caml_string_true : forall s: string, caml_string_eqb (caml_string_of_chars s) (caml_string_of_chars s) = true.
+Lemma caml_string_eqb_true : forall s: string, caml_string_eqb (caml_string_of_chars s) (caml_string_of_chars s) = true.
+Admitted.
+Lemma caml_string_eqb_false : forall s1 s2: string, s1 <> s2 -> caml_string_eqb (caml_string_of_chars s1) (caml_string_of_chars s2) = false.
 Admitted.
 
-Lemma int_parses_corr : parses IntParser 2 (caml_string_of_chars "start") = true.
+Definition bad_env : Environment.environment tag_t := nil.
+
+Lemma int_parses_fail : parses IntParser 2 (caml_string_of_chars "start") bad_env = false.
 Proof.
+
+  unfold IntParser.
+  unfold states.
+  unfold start_st.
   unfold parses.
-  unfold step_trans.
-  unfold step. unfold run_with_state.
-  unfold IntParser. auto. unfold lookup_state.
-  unfold states. unfold start_st. auto.
-  rewrite caml_string_true.
-  unfold body. auto. 
-  unfold eval_statement.
-  unfold Monad.mbind. auto.
+  unfold step_trans. auto.
+  unfold run_with_state.
+  unfold step. auto.
+  unfold lookup_state.
+
+  rewrite caml_string_eqb_true. 
+  auto.
+  (* reflexivity. *)
+Qed.
+
+Definition pkt_value : Value tag_t := ValObj _ (ValObjPacket _ (true :: true :: nil)).
+Definition out_value : Value tag_t := ValBase _ (ValBaseInteger _ 0).
+Definition top_scope : Environment.scope tag_t := 
+  Environment.extend_scope _ (caml_string_of_chars "pkt") pkt_value (
+    Environment.extend_scope _ (caml_string_of_chars "output") out_value (
+      Environment.MStr.empty _
+    )
+  ).
+
+Definition inter_scope : Environment.scope tag_t := 
+  Environment.MStr.add (caml_string_of_chars "pkt")
+                              (ValObj tag_t (ValObjPacket tag_t nil))
+                              top_scope.
+Definition good_env : Environment.environment tag_t := top_scope :: nil.
+
+Compute Environment.MStr.find. 
+Compute Environment.MStr.find (caml_string_of_chars "pkt") top_scope.
+
+Lemma top_find_pkt : Environment.MStr.find (caml_string_of_chars "pkt") top_scope = Some pkt_value.
 Admitted.
+Lemma top_find_val : Environment.MStr.find (caml_string_of_chars "output") top_scope = Some out_value.
+Admitted.
+Lemma top_find_val_inter : Environment.MStr.find (caml_string_of_chars "output") inter_scope = Some out_value.
+Admitted.
+
+
+Lemma int_parses : parses IntParser 2 (caml_string_of_chars "start") good_env = true.
+Proof.
+  unfold IntParser.
+  unfold states.
+  unfold start_st.
+  unfold parses.
+  unfold step_trans. auto.
+  unfold run_with_state.
+  unfold good_env.
+  unfold Monad.mbind.
+  unfold state_monad_inst.
+  unfold state_bind.
+
+  unfold step.
+  unfold lookup_state.
+  rewrite caml_string_eqb_true.
+  unfold Monad.mbind. unfold state_monad_inst. unfold state_bind.
+  unfold body. 
+
+  unfold eval_statement.
+  unfold Monad.mbind. unfold state_monad_inst. unfold state_bind.
+  unfold Environment.map_env. unfold Environment.push_scope. unfold Environment.extend_scope.
+  auto.
+  unfold Monad.mret. unfold state_monad_inst. unfold state_return.
+
+  unfold states_to_block. unfold List.fold_right.
+  unfold extract_stmt.
+
+  unfold eval_method_call.
+  unfold eval_expression. unfold pkt_extract_expr.
+  unfold Environment.find_environment. unfold Environment.lift_env_lookup_fn.
+  unfold Monad.mbind. unfold state_monad_inst. unfold state_bind.
+  unfold Environment.toss_value.
+  unfold Environment.find_environment'.
+  unfold Environment.str_of_name_warning_not_safe.
+  auto.
+  assert (H := top_find_pkt).
+  unfold Environment.MStr.find. unfold Environment.MStr.Raw.find. auto.
+  unfold Environment.MStr.this. 
+  unfold Environment.MStr.empty. unfold Environment.MStr.Raw.empty.
+  
+  unfold Environment.MStr.find in H. unfold Environment.MStr.Raw.find in H. 
+
+  unfold Environment.MStr.this in H.
+  rewrite H.
+  clear H.
+
+  unfold Monad.mret. unfold state_monad_inst. unfold state_return.
+  unfold pkt_value.
+  unfold StrConstants.extract.
+
+  rewrite caml_string_eqb_true.
+  unfold extract_value_func. unfold eval_builtin_func.
+
+  unfold Monad.mbind. unfold state_monad_inst. unfold state_bind.
+  unfold eval_arguments.
+  unfold Monad.mbind. unfold state_monad_inst. unfold state_bind.
+  unfold eval_expression. unfold output_expr.
+
+  unfold Environment.find_environment. unfold Environment.lift_env_lookup_fn. unfold Environment.find_lvalue'.
+  unfold Environment.find_environment'. unfold Environment.str_of_name_warning_not_safe.
+  
+  unfold Environment.MStr.find. unfold Environment.MStr.Raw.find. auto.
+
+  unfold Environment.MStr.this.
+  assert (H := top_find_val).
+
+  unfold Environment.MStr.find in H. unfold Environment.MStr.Raw.find in H. auto.
+
+  unfold Environment.MStr.this in H.
+  rewrite H. clear H.
+
+  unfold Monad.mret. unfold state_monad_inst. unfold state_return.
+
+  unfold StrConstants.extract. 
+  unfold StrConstants.isValid. rewrite caml_string_eqb_false.
+  unfold StrConstants.setValid. rewrite caml_string_eqb_false.
+  unfold StrConstants.setInvalid. rewrite caml_string_eqb_false.
+  unfold StrConstants.pop_front. rewrite caml_string_eqb_false.
+  unfold StrConstants.push_front. rewrite caml_string_eqb_false.
+  unfold is_packet_func.
+  unfold StrConstants.extract. rewrite caml_string_eqb_true.
+
+  unfold Environment.dummy_value.
+  unfold eval_packet_func.
+  unfold Monad.mbind. unfold state_monad_inst. unfold state_bind.
+  unfold Environment.find_lvalue. unfold Environment.lift_env_lookup_fn. unfold Environment.find_lvalue'.
+  unfold Environment.find_environment'. unfold Environment.str_of_name_warning_not_safe.
+  unfold Environment.MStr.this.
+  unfold Environment.MStr.find. unfold Environment.MStr.Raw.find. auto.
+
+  unfold Environment.MStr.this.
+
+  assert (H := top_find_pkt).
+  unfold Environment.MStr.find in H. unfold Environment.MStr.Raw.find in H.
+  unfold Environment.MStr.this in H.
+  rewrite H. clear H.
+
+  unfold Monad.mret. unfold state_monad_inst. unfold state_return.
+
+  unfold pkt_value.
+  unfold StrConstants.extract. rewrite caml_string_eqb_true.
+  unfold Packet.eval_packet_extract_fixed.
+  unfold out_type.
+
+  unfold Monad.mbind. unfold state_monad_inst. unfold state_bind.
+  unfold Packet.read_first_bits.
+  unfold Monad.mret. unfold state_monad_inst. unfold state_return.
+
+
+  unfold Environment.update_lvalue. unfold Environment.lift_env_fn. unfold Environment.update_lvalue'.
+  
+  unfold Environment.update_environment'.
+  unfold Environment.str_of_name_warning_not_safe.
+  unfold Environment.MStr.find. unfold Environment.MStr.Raw.find. unfold Environment.MStr.this.
+
+
+  unfold Monad.mbind. unfold state_monad_inst. unfold state_bind.
+
+  assert (H := top_find_pkt).
+  unfold Environment.MStr.find in H. unfold Environment.MStr.Raw.find in H.
+  unfold Environment.MStr.this in H.
+  rewrite H. clear H.
+  unfold Option.option_monad_inst. unfold Option.option_bind.
+  (* unfold Environment.update_scope. *)
+  unfold Environment.insert_scope.
+
+  unfold Monad.mbind. unfold Option.option_monad_inst. unfold Option.option_bind.
+
+  rewrite top_find_pkt.
+
+  unfold Monad.mret. unfold Option.option_ret. unfold state_return.
+
+  unfold eval_lvalue.
+  unfold Monad.mret. unfold state_monad_inst. unfold state_return.
+
+  assert (H := top_find_val_inter).
+  unfold Environment.MStr.find in H. unfold Environment.MStr.Raw.find in H. unfold Environment.MStr.this in H.
+  unfold inter_scope in H.
+  rewrite H. clear H.
+  assert (H := top_find_val_inter).
+  unfold inter_scope in H.
+  rewrite H. clear H.
+
+  unfold Environment.pop_scope.
+  unfold eval_transition.
+  unfold Monad.mret. unfold state_monad_inst. unfold state_return.
+  unfold StrConstants.accept. 
+  rewrite caml_string_eqb_true.
+  auto.
+  rewrite <- String.eqb_neq. auto.
+  rewrite <- String.eqb_neq. auto.
+  rewrite <- String.eqb_neq. auto.
+  rewrite <- String.eqb_neq. auto.
+  rewrite <- String.eqb_neq. auto.
+Qed.
+
